turboflow finished, with an implementation bug found and fixed

newLibrary/finished_examples/turboflow.dfy
@@ -1,35 +1,96 @@
 /*
-
 This implements the data plane cache of TurboFlow. 
 
 TurboFlow is a flow telemetry system with two components: 
-    - a Data plane cache measures per-flow flow metrics (e.g., total packet count) 
+    - a Data plane cache measures per-flow flow counters (e.g., total packet count) 
       over short time intervals. When the cache evicts a flow, 
-      it sends a record of its current aggregate metrics to a collection server.       
+      it sends a record of the cached value of that flow's counter to 
+      a backend collection server. 
     - The collection server aggregates records from the cache to calculate 
-      per-flow metrics for the entire duration of every flow. 
+      the complete per flow counters.
 
-The main property of the data plane cache is: 
-    For every flow that has been seen by the cache, 
-    the counter in the cache + the sum of the counts sent to the server 
-    = the true total count of the flow
+The main property of the data plane cache is a per flow property:
+    For every flow that has been seen by the system, 
+    the counter in the cache + the counter in the collector 
+    is equal to the true total count of the flow.
 
-Idea: 
-Thinking about correctness, TurboFlow is susceptible to packet loss... 
-Can we make a stronger implementation that is robust against it to some degree?
+The verification strategy is to keep models of the collector and a 
+"reference" store. The reference store counts all the packets. 
+We verify the cach + collector count is the same as the reference count.
+
+This property did not hold in the initial version of TurboFlow, 
+because it does not deal with counter overflows in the cache.
+To fix this, we add the extra exception handling case 
+around line 186, where we evict a flow if its counter is in 
+danger of overflowing on the next packet. 
+
+We also add an assumption that packet lengths are always 
+under a certain value.
+
+We can also probably find bugs in TurboFlow related to: 
+    - timestamp / duration overflows
+    - packet loss
 */
 
 
 include "verifiableLucid.dfy"
 
 module BloomFilter refines VerifiableLucid {
+    const nFlows : nat := 1024
+    type  flowIdx_t = f : nat | f < 1024
+    type  flowKey_t = (uint32, uint32)
+    const maxPktLen : uint32 := 2048
+
+    class ExactStore {
+        ghost var flows : map<flowKey_t, nat>
+        ghost constructor () 
+            ensures fresh(this)
+            ensures flows == map[]
+        {
+            flows := map[];
+        }
+
+        ghost method Update(key : flowKey_t, len : uint32)
+            modifies this`flows
+            ensures flows.Keys == old(flows).Keys + {key} // all old flows are still here, and the new flow too
+            // all counters besides for key stay the same
+            ensures forall k | k in old(flows) :: k in flows && (k != key ==> old(flows)[k] == flows[k])
+            // flows[key] is incremented appropriately
+            ensures if key in old(flows)
+                        then key in flows && flows[key] == old(flows)[key] + len
+                        else flows[key] == len
+            
+        {
+            flows := 
+                if (key in flows) then
+                    flows[key := flows[key] + len]
+                else
+                    flows[key := len];
+        }
+    }
+
+    function incr (oldVal: uint32, incrBy: uint32) : uint32 { 
+        to_uint32(oldVal + incrBy)
+    }
+
+    function safeIncr (oldVal: uint32, incrBy: uint32) : uint32 {         
+        // if the new counter value is above some unsafe threshold, 
+        // such that the next packet may cause it to overflow, 
+        // we want to evict, which means resetting it.
+        if ((oldVal + incrBy) % max32) >= max32 - maxPktLen
+        then incrBy
+        else to_uint32(oldVal + incrBy)
+    }
+
+
+    function memval (oldVal: uint32, unused: uint32) : uint32 { oldVal }
+    function newval (oldVal: uint32, newVal: uint32) : uint32 { newVal }
 
     datatype Event = 
         | Packet(src : uint32, dst : uint32, len : uint32)
         | FlowRecord(src : uint32, dst : uint32, len : uint32)
 
     class Program ... {
-        const nFlows : nat := 1024
         const seed : nat := 7
         const collectorPort : nat := 0
 
@@ -46,49 +107,95 @@ module BloomFilter refines VerifiableLucid {
             // Non-aliasing
             && srcs != dsts && srcs != lens && dsts != lens
             // array lengths
-            && |srcs.cells| == |dsts.cells| == |lens.cells| == 1024
+            && |srcs.cells| == |dsts.cells| == |lens.cells| == nFlows
+            // ghost aliasing ARGH
+            && this.fullStore != this.collectorStore
         }
 
+        ghost var fullStore : ExactStore // models collector that just processes everything
+        ghost var collectorStore : ExactStore // models collector that processes evicted records
+
         constructor ()
-        ensures ValidArrays()
+            ensures ValidArrays()
+            ensures fullStore.flows == map[]
+            ensures collectorStore.flows == map[]
         {
             srcs := new LArray<uint32>.Create(nFlows, 0);
             dsts := new LArray<uint32>.Create(nFlows, 0);
             lens := new LArray<uint32>.Create(nFlows, 0);
             ArrayRepr := {srcs, dsts, lens};
+            fullStore := new ExactStore();
+            collectorStore := new ExactStore();
         }
 
-        // memops
-        function incr (oldVal: uint32, incrBy: uint32) : uint32 { 
-            to_uint32(oldVal + incrBy) 
+        function cacheLen(key : flowKey_t) : nat
+            reads this, ArrayRepr
+            requires ValidArrays()
+        {
+            var idx : uint32 := hashn(10, seed, [key.0, key.1]);
+            if ((srcs.cells[idx] == key.0) && (dsts.cells[idx] == key.1))
+            then lens.cells[idx]
+            else 0
         }
-        function memval (oldVal: uint32, unused: uint32) : uint32 { oldVal }
-        function newval (oldVal: uint32, newVal: uint32) : uint32 { newVal }
+        ghost function collectorLen(key : flowKey_t) : nat            
+            reads this`collectorStore, this.collectorStore
+        {
+            if key in this.collectorStore.flows
+                then this.collectorStore.flows[key]
+                else 0 // not found
+        }
 
+        ghost function fullLen(key : flowKey_t) : nat
+            reads this`fullStore, this.fullStore
+        {            
+            if key in fullStore.flows
+                then fullStore.flows[key]
+                else 0               
+        }
+
+        ghost predicate stateInvariant(key : flowKey_t)
+            // The cache is correct for flow k if the cache counter + collector counter == full counter
+            reads this, ArrayRepr
+            reads this.fullStore, this.collectorStore
+            requires ValidArrays()            
+        {
+            fullLen(key) == cacheLen(key) + collectorLen(key)
+        }
 
         method packet(src : uint32, dst : uint32, len : uint32)
             modifies srcs`cells, dsts`cells, lens`cells, this`emittedEvents
+            modifies this.fullStore, this.collectorStore // ghost
+            requires this.fullStore != this.collectorStore
             requires ValidArrays()
+            requires len < maxPktLen && cacheLen((src, dst)) < max32 - maxPktLen // Length correctness
+            requires stateInvariant((src, dst))
             ensures  ValidArrays()
-            // Left off here. Add the proof and ensures clause that the sum of the length, 
-            // for every flow, is actually equal to the total length of the flow.
-            // We will probably have to deal with rollovers of the counter!
+            ensures  cacheLen((src, dst)) < max32 - maxPktLen
+            ensures  stateInvariant((src, dst))
+            // Without the additional case that checks for a near-overflow and then evicts, 
+            // only the weaker state invariant below holds
+            // ensures  (old(cacheLen((src, dst))) + len as nat < max32) ==> stateInvariant((src, dst))
         {
+            fullStore.Update((src, dst), len);
             var idx : uint32 := hashn(10, seed, [src, dst]);
             assert (idx < nFlows);
-            // update key arrays and get old values
+
             var oldSrc := LArray<uint32>.Update(srcs, idx, memval, 0, newval, src);
-            var oldDst := LArray<uint32>.Update(dsts, idx, memval, 0, newval, dst);
-            // check for collision
+            var oldDst := LArray<uint32>.Update(dsts, idx, memval, 0, newval, dst);         
+
+            // check for collision and reset the counter if there is one.
             if (oldSrc != src || oldDst != dst) {
-                // collision -- reset len[idx]
                 var oldLen := LArray<uint32>.Update(lens, idx, memval, 0, newval, len);
-                // since there was a collision, we have to generate a record event to collector
                 generate_port(collectorPort, FlowRecord(oldSrc, oldDst, oldLen));
+                collectorStore.Update((oldSrc, oldDst), oldLen);
             }
             else {
-                // no collision -- just increment len[idx]
-                LArray<uint32>.Set(lens, idx, incr, len);
+                var oldLen : uint32 := LArray<uint32>.Update(lens, idx, memval, 0, safeIncr, len);
+                // if the old length was too large, reset the counter.
+                if ((oldLen + len)% max32 >= max32 - maxPktLen) {
+                    generate_port(collectorPort, FlowRecord(oldSrc, oldDst, oldLen));
+                    collectorStore.Update((oldSrc, oldDst), oldLen);
+                }
             }
         }
     }
